Updates.

FOL/NV/Sub/Var/All/Ind/ReplaceFree.lean
@@ -11,148 +11,148 @@ open Formula_
 
 
 /--
-  IsReplaceFree σ F F' := True if and only if F' is the result of the simultaneous replacement of each free occurrence of any variable v in the formula F by σ v.
+  is_replace_free_var_all_ind σ F F' := True if and only if F' is the result of the simultaneous replacement of each free occurrence of any variable v in the formula F by σ v.
 -/
-inductive IsReplaceFree : (VarName_ → VarName_) → Formula_ → Formula_ → Prop
+inductive is_replace_free_var_all_ind : (VarName_ → VarName_) → Formula_ → Formula_ → Prop
 
   | pred_const_
     (σ : VarName_ → VarName_)
     (X : PredName_)
     (xs : List VarName_) :
-    IsReplaceFree σ (pred_const_ X xs) (pred_const_ X (xs.map σ))
+    is_replace_free_var_all_ind σ (pred_const_ X xs) (pred_const_ X (xs.map σ))
 
   | pred_var_
     (σ : VarName_ → VarName_)
     (X : PredName_)
     (xs : List VarName_) :
-    IsReplaceFree σ (pred_var_ X xs) (pred_var_ X (xs.map σ))
+    is_replace_free_var_all_ind σ (pred_var_ X xs) (pred_var_ X (xs.map σ))
 
   | eq_
     (σ : VarName_ → VarName_)
     (x y : VarName_) :
-    IsReplaceFree σ (eq_ x y) (eq_ (σ x) (σ y))
+    is_replace_free_var_all_ind σ (eq_ x y) (eq_ (σ x) (σ y))
 
   | true_
     (σ : VarName_ → VarName_) :
-    IsReplaceFree σ true_ true_
+    is_replace_free_var_all_ind σ true_ true_
 
   | false_
     (σ : VarName_ → VarName_) :
-    IsReplaceFree σ false_ false_
+    is_replace_free_var_all_ind σ false_ false_
 
   | not_
     (σ : VarName_ → VarName_)
     (phi : Formula_)
     (phi' : Formula_) :
-    IsReplaceFree σ phi phi' →
-    IsReplaceFree σ phi.not_ phi'.not_
+    is_replace_free_var_all_ind σ phi phi' →
+    is_replace_free_var_all_ind σ phi.not_ phi'.not_
 
   | imp_
     (σ : VarName_ → VarName_)
     (phi psi : Formula_)
     (phi' psi' : Formula_) :
-    IsReplaceFree σ phi phi' →
-    IsReplaceFree σ psi psi' →
-    IsReplaceFree σ (phi.imp_ psi) (phi'.imp_ psi')
+    is_replace_free_var_all_ind σ phi phi' →
+    is_replace_free_var_all_ind σ psi psi' →
+    is_replace_free_var_all_ind σ (phi.imp_ psi) (phi'.imp_ psi')
 
   | and_
     (σ : VarName_ → VarName_)
     (phi psi : Formula_)
     (phi' psi' : Formula_) :
-    IsReplaceFree σ phi phi' →
-    IsReplaceFree σ psi psi' →
-    IsReplaceFree σ (phi.and_ psi) (phi'.and_ psi')
+    is_replace_free_var_all_ind σ phi phi' →
+    is_replace_free_var_all_ind σ psi psi' →
+    is_replace_free_var_all_ind σ (phi.and_ psi) (phi'.and_ psi')
 
   | or_
     (σ : VarName_ → VarName_)
     (phi psi : Formula_)
     (phi' psi' : Formula_) :
-    IsReplaceFree σ phi phi' →
-    IsReplaceFree σ psi psi' →
-    IsReplaceFree σ (phi.or_ psi) (phi'.or_ psi')
+    is_replace_free_var_all_ind σ phi phi' →
+    is_replace_free_var_all_ind σ psi psi' →
+    is_replace_free_var_all_ind σ (phi.or_ psi) (phi'.or_ psi')
 
   | iff_
     (σ : VarName_ → VarName_)
     (phi psi : Formula_)
     (phi' psi' : Formula_) :
-    IsReplaceFree σ phi phi' →
-    IsReplaceFree σ psi psi' →
-    IsReplaceFree σ (phi.iff_ psi) (phi'.iff_ psi')
+    is_replace_free_var_all_ind σ phi phi' →
+    is_replace_free_var_all_ind σ psi psi' →
+    is_replace_free_var_all_ind σ (phi.iff_ psi) (phi'.iff_ psi')
 
   | forall_
     (σ : VarName_ → VarName_)
     (x : VarName_)
     (phi phi' : Formula_) :
-    IsReplaceFree (Function.updateITE σ x x) phi phi' →
-    IsReplaceFree σ (forall_ x phi) (forall_ x phi')
+    is_replace_free_var_all_ind (Function.updateITE σ x x) phi phi' →
+    is_replace_free_var_all_ind σ (forall_ x phi) (forall_ x phi')
 
   | exists_
     (σ : VarName_ → VarName_)
     (x : VarName_)
     (phi phi' : Formula_) :
-    IsReplaceFree (Function.updateITE σ x x) phi phi' →
-    IsReplaceFree σ (exists_ x phi) (exists_ x phi')
+    is_replace_free_var_all_ind (Function.updateITE σ x x) phi phi' →
+    is_replace_free_var_all_ind σ (exists_ x phi) (exists_ x phi')
 
   | def_
     (σ : VarName_ → VarName_)
     (X : DefName_)
     (xs : List VarName_) :
-    IsReplaceFree σ (def_ X xs) (def_ X (xs.map σ))
+    is_replace_free_var_all_ind σ (def_ X xs) (def_ X (xs.map σ))
 
 
 example
   (F F' : Formula_)
   (σ : VarName_ → VarName_)
   (h1 : Rec.fast_replace_free_var_all_rec σ F = F') :
-  IsReplaceFree σ F F' :=
+  is_replace_free_var_all_ind σ F F' :=
   by
   subst h1
   induction F generalizing σ
   all_goals
     simp only [Rec.fast_replace_free_var_all_rec]
   case pred_const_ X xs =>
-    apply IsReplaceFree.pred_const_
+    apply is_replace_free_var_all_ind.pred_const_
   case pred_var_ X xs =>
-    apply IsReplaceFree.pred_var_
+    apply is_replace_free_var_all_ind.pred_var_
   case eq_ x y =>
-    apply IsReplaceFree.eq_
+    apply is_replace_free_var_all_ind.eq_
   case true_ =>
-    apply IsReplaceFree.true_
+    apply is_replace_free_var_all_ind.true_
   case false_ =>
-    apply IsReplaceFree.false_
+    apply is_replace_free_var_all_ind.false_
   case not_ phi phi_ih =>
-    apply IsReplaceFree.not_
+    apply is_replace_free_var_all_ind.not_
     apply phi_ih
   case imp_ phi psi phi_ih psi_ih =>
-    apply IsReplaceFree.imp_
+    apply is_replace_free_var_all_ind.imp_
     · apply phi_ih
     · apply psi_ih
   case and_ phi psi phi_ih psi_ih =>
-    apply IsReplaceFree.and_
+    apply is_replace_free_var_all_ind.and_
     · apply phi_ih
     · apply psi_ih
   case or_ phi psi phi_ih psi_ih =>
-    apply IsReplaceFree.or_
+    apply is_replace_free_var_all_ind.or_
     · apply phi_ih
     · apply psi_ih
   case iff_ phi psi phi_ih psi_ih =>
-    apply IsReplaceFree.iff_
+    apply is_replace_free_var_all_ind.iff_
     · apply phi_ih
     · apply psi_ih
   case forall_ x phi phi_ih =>
-    apply IsReplaceFree.forall_
+    apply is_replace_free_var_all_ind.forall_
     apply phi_ih
   case exists_ x phi phi_ih =>
-    apply IsReplaceFree.exists_
+    apply is_replace_free_var_all_ind.exists_
     · apply phi_ih
   case def_ X xs =>
-    apply IsReplaceFree.def_
+    apply is_replace_free_var_all_ind.def_
 
 
 example
   (F F' : Formula_)
   (σ : VarName_ → VarName_)
-  (h1 : IsReplaceFree σ F F') :
+  (h1 : is_replace_free_var_all_ind σ F F') :
   Rec.fast_replace_free_var_all_rec σ F = F' :=
   by
   induction h1
